safechecker/theories/PCUICWfEnv.v
@@ -11,39 +11,42 @@ Definition on_global_decls_dec {cf:checker_flags} :=
   on_global_decls_data cumulSpec0 (lift_typing typing) (cf:=cf).
 
 Class abstract_env_struct {cf:checker_flags} (abstract_env_impl abstract_env_ext_impl : Type) := {
-  abstract_env_lookup : abstract_env_ext_impl -> kername -> option global_decl;
-  abstract_env_ext_retroknowledge : abstract_env_ext_impl -> Retroknowledge.t;
-  abstract_env_conv_pb_relb : abstract_env_ext_impl -> conv_pb -> Universe.t -> Universe.t -> bool;
-  abstract_env_compare_global_instance : abstract_env_ext_impl -> (Universe.t -> Universe.t -> bool) -> global_reference -> nat -> list Level.t -> list Level.t -> bool;
-  abstract_env_level_mem : abstract_env_ext_impl -> Level.t -> bool;
-  abstract_env_ext_wf_universeb : abstract_env_ext_impl -> Universe.t -> bool;
-  abstract_env_check_constraints : abstract_env_ext_impl -> ConstraintSet.t -> bool;
-  abstract_env_guard : abstract_env_ext_impl -> FixCoFix -> context -> mfixpoint term -> bool;
-  abstract_env_fixguard X := abstract_env_guard X Fix;
-  abstract_env_cofixguard X := abstract_env_guard X CoFix;
-  abstract_env_empty : abstract_env_impl;
-  abstract_env_init (cs:ContextSet.t) (retro : Retroknowledge.t) : on_global_univs cs -> abstract_env_impl;
-  abstract_env_univ : abstract_env_impl -> ContextSet.t;
-  abstract_env_global_declarations : abstract_env_impl -> global_declarations;
-  abstract_env_retroknowledge : abstract_env_impl -> Retroknowledge.t;
-  abstract_env_add_decl X (kn:kername) (d:global_decl) :
-   ∥ on_global_decls_dec (abstract_env_univ X) (abstract_env_retroknowledge X) (abstract_env_global_declarations X) kn d ∥ -> abstract_env_impl;
-  abstract_env_empty_ext : abstract_env_impl -> abstract_env_ext_impl;
-  abstract_env_is_consistent : VSet.t * GoodConstraintSet.t -> bool ;
-  abstract_env_is_consistent_uctx : abstract_env_impl -> VSet.t * GoodConstraintSet.t -> bool ;
-  abstract_env_add_uctx X uctx udecl :
-    gc_of_uctx (uctx_of_udecl udecl) = Some uctx ->
-    ∥ on_udecl (abstract_env_univ X) udecl ∥ ->
-    abstract_env_ext_impl ;
-  abstract_pop_decls : abstract_env_impl -> abstract_env_impl ;
-
   (* This part of the structure is here to state the correctness properties *)
 
   abstract_env_rel : abstract_env_impl -> global_env -> Prop;
   abstract_env_ext_rel : abstract_env_ext_impl -> global_env_ext -> Prop;
 
+  (* Operations on the environment *)
+
+  abstract_env_lookup : abstract_env_ext_impl -> kername -> option global_decl;
+  abstract_env_empty : abstract_env_impl;
+  abstract_env_init (cs:ContextSet.t) (retro : Retroknowledge.t) : on_global_univs cs -> abstract_env_impl;
+  abstract_env_add_decl X (kn:kername) (d:global_decl) :
+   (forall Σ : global_env, abstract_env_rel X Σ -> ∥ on_global_decls_dec Σ.(universes) Σ.(retroknowledge) Σ.(declarations) kn d ∥) 
+   -> abstract_env_impl;
+  abstract_env_empty_ext : abstract_env_impl -> abstract_env_ext_impl;
+  abstract_env_add_uctx X uctx udecl :
+    gc_of_uctx (uctx_of_udecl udecl) = Some uctx ->
+    (forall Σ : global_env, abstract_env_rel X Σ -> ∥ on_udecl Σ.(universes) udecl ∥) ->
+    abstract_env_ext_impl ;
+  abstract_pop_decls : abstract_env_impl -> abstract_env_impl ;
   abstract_make_wf_env_ext : forall (X:abstract_env_impl) (univs : universes_decl)
     (prf : forall Σ : global_env, abstract_env_rel X Σ -> ∥ wf_ext (Σ, univs) ∥), abstract_env_ext_impl ;
+  abstract_primitive_constant : abstract_env_ext_impl -> Primitive.prim_tag -> option kername;
+
+    (* Primitive decision procedures *)
+
+  abstract_env_conv_pb_relb : abstract_env_ext_impl -> conv_pb -> Universe.t -> Universe.t -> bool;
+  abstract_env_compare_global_instance : abstract_env_ext_impl -> (Universe.t -> Universe.t -> bool) -> global_reference -> nat -> list Level.t -> list Level.t -> bool;
+  abstract_env_level_mem : abstract_env_ext_impl -> LevelSet.t -> Level.t -> bool;
+  abstract_env_ext_wf_universeb : abstract_env_ext_impl -> Universe.t -> bool;
+  abstract_env_check_constraints : abstract_env_ext_impl -> ConstraintSet.t -> bool;
+  abstract_env_guard : abstract_env_ext_impl -> FixCoFix -> context -> mfixpoint term -> bool;
+  abstract_env_fixguard X := abstract_env_guard X Fix;
+  abstract_env_cofixguard X := abstract_env_guard X CoFix;
+  abstract_env_is_consistent : VSet.t * GoodConstraintSet.t -> bool ;
+  abstract_env_is_consistent_uctx : abstract_env_impl -> VSet.t * GoodConstraintSet.t -> bool ;
+
 }.
 
 Definition abstract_env_eq {cf:checker_flags} {abstract_env_impl abstract_env_ext_impl : Type} `{!abstract_env_struct abstract_env_impl abstract_env_ext_impl}
@@ -60,25 +63,24 @@ Class abstract_env_prop {cf:checker_flags} (abstract_env_impl abstract_env_ext_i
       abstract_env_ext_rel X Σ -> abstract_env_ext_rel X Σ' ->  Σ = Σ';
    abstract_env_lookup_correct X {Σ} c : abstract_env_ext_rel X Σ ->
       lookup_env Σ c = abstract_env_lookup X c ;
-   abstract_env_ext_retroknowledge_correct X {Σ : global_env_ext} (wfΣ : abstract_env_ext_rel X Σ) :
-      Σ.(retroknowledge) = abstract_env_ext_retroknowledge X ;
   abstract_env_compare_universe_correct X {Σ} (wfΣ : abstract_env_ext_rel X Σ) conv_pb u u' :
         wf_universe Σ u -> wf_universe Σ u' ->
         compare_universe conv_pb Σ u u' <->
         abstract_env_conv_pb_relb X conv_pb u u';
-    abstract_env_compare_global_instance_correct X {Σ} (wfΣ : abstract_env_ext_rel X Σ) R leq ref n l l' :
+  abstract_env_compare_global_instance_correct X {Σ} (wfΣ : abstract_env_ext_rel X Σ) R leq ref n l l' :
       (forall u u', wf_universe Σ u -> wf_universe Σ u' -> reflect (R u u') (leq u u')) ->
       wf_universe_instance Σ l ->
       wf_universe_instance Σ l' ->
       R_global_instance Σ (eq_universe Σ) R ref n l l' <->
       abstract_env_compare_global_instance X leq ref n l l' ;
-    abstract_env_level_mem_correct X {Σ} (wfΣ : abstract_env_ext_rel X Σ) u : level_mem Σ u = abstract_env_level_mem X u;
-    abstract_env_ext_wf_universeb_correct X_ext {Σ} (wfΣ : abstract_env_ext_rel X_ext Σ) u :
+  abstract_env_level_mem_correct X {Σ} (wfΣ : abstract_env_ext_rel X Σ) levels u : 
+    LevelSet.mem u (LevelSet.union levels (global_ext_levels Σ)) = abstract_env_level_mem X levels u;
+  abstract_env_ext_wf_universeb_correct X_ext {Σ} (wfΣ : abstract_env_ext_rel X_ext Σ) u :
       wf_universeb Σ u = abstract_env_ext_wf_universeb X_ext u;
-    abstract_env_check_constraints_correct X {Σ} (wfΣ : abstract_env_ext_rel X Σ) ctrs :
+  abstract_env_check_constraints_correct X {Σ} (wfΣ : abstract_env_ext_rel X Σ) ctrs :
       check_univs -> uctx_invariants ((global_ext_uctx Σ).1, ctrs) ->
       valid_constraints Σ ctrs <-> abstract_env_check_constraints X ctrs;
-    abstract_env_guard_correct X {Σ} (wfΣ : abstract_env_ext_rel X Σ) fix_cofix Γ mfix :
+  abstract_env_guard_correct X {Σ} (wfΣ : abstract_env_ext_rel X Σ) fix_cofix Γ mfix :
       guard fix_cofix Σ Γ mfix <-> abstract_env_guard X fix_cofix Γ mfix;
   abstract_env_exists X : ∥ ∑ Σ , abstract_env_rel X Σ ∥;
   abstract_env_wf X {Σ} : abstract_env_rel X Σ -> ∥ wf Σ ∥;
@@ -87,10 +89,7 @@ Class abstract_env_prop {cf:checker_flags} (abstract_env_impl abstract_env_ext_i
   abstract_env_empty_ext_rel X {Σ} :
     (abstract_env_rel X Σ.1 /\ Σ.2 = Monomorphic_ctx)  <->
     abstract_env_ext_rel (abstract_env_empty_ext X) Σ ;
-    abstract_env_global_declarations_correct X {Σ} :
-    abstract_env_rel X Σ ->
-      declarations Σ = abstract_env_global_declarations X ;
-    abstract_env_init_correct univs retro cuniv :
+  abstract_env_init_correct univs retro cuniv :
     abstract_env_rel (abstract_env_init univs retro cuniv)
     {| universes := univs; declarations := []; retroknowledge := retro |} ;
   abstract_env_add_decl_correct X Σ kn d H : abstract_env_rel X Σ ->
@@ -110,10 +109,6 @@ Class abstract_env_prop {cf:checker_flags} (abstract_env_impl abstract_env_ext_i
     (consistent ((Σ,udecl):global_env_ext) /\
        consistent_extension_on (global_uctx Σ) (uctx_of_udecl udecl).2)
     <-> abstract_env_is_consistent_uctx X uctx ;
-  abstract_env_univ_correct X {Σ} (wfΣ : abstract_env_rel X Σ) :
-    (Σ:ContextSet.t) = abstract_env_univ X ;
-  abstract_env_retroknowledge_correct X {Σ : global_env} (wfΣ : abstract_env_rel X Σ) :
-    Σ.(retroknowledge) = abstract_env_retroknowledge X ;
   abstract_pop_decls_correct X decls (prf : forall Σ : global_env, abstract_env_rel X Σ ->
             exists d, Σ.(declarations) = d :: decls) :
     let X' := abstract_pop_decls X in
@@ -122,7 +117,9 @@ Class abstract_env_prop {cf:checker_flags} (abstract_env_impl abstract_env_ext_i
                       Σ.(retroknowledge) = Σ'.(retroknowledge);
   abstract_make_wf_env_ext_correct X univs prf :
     let X' := abstract_make_wf_env_ext X univs prf in
-    forall Σ Σ', abstract_env_rel X Σ -> abstract_env_ext_rel X' Σ' -> Σ' = (Σ, univs)
+    forall Σ Σ', abstract_env_rel X Σ -> abstract_env_ext_rel X' Σ' -> Σ' = (Σ, univs);
+  abstract_primitive_constant_correct X tag Σ :
+    abstract_env_ext_rel X Σ -> abstract_primitive_constant X tag = PCUICEnvironment.primitive_constant Σ tag
   }.
 
 Definition abstract_env_impl {cf:checker_flags} := ∑ X Y Z, @abstract_env_prop _ X Y Z.
